Common.v
@@ -39,36 +39,60 @@ Fixpoint mem x xs :=
   | x' :: xs' => if x =? x' then true else mem x xs'
   end.
 
-Lemma not_in_implies_mem_false :
+Lemma not_in_iff_mem_false :
   forall x xs,
-    ~ (In x xs) -> mem x xs = false.
+    ~ (In x xs) <-> mem x xs = false.
 Proof.
-  intros.
-  induction xs.
-  - reflexivity.
-  - simpl.
-    apply not_in_cons in H. destruct H.
-    unfold not in H.
-    destruct (x =? a) eqn:Heq_xa.
-    + exfalso. apply beq_nat_true in Heq_xa.
-      apply H. apply Heq_xa.
-    + apply IHxs. apply H0.
+  intros. split.
+  - intro Hxs. induction xs.
+    + auto.
+    + simpl.
+      apply not_in_cons in Hxs. destruct Hxs.
+      unfold not in H.
+      destruct (x =? a) eqn:Heq_xa.
+      * exfalso. apply beq_nat_true in Heq_xa.
+        apply H. apply Heq_xa.
+      * apply IHxs. apply H0.
+  - intro Hxs. induction xs.
+    + auto.
+    + destruct (x =? a) eqn:Heq_xa.
+      * apply not_in_cons.
+        split;
+          unfold mem in Hxs; rewrite Heq_xa in Hxs;
+          discriminate Hxs.
+      * apply not_in_cons. split.
+        ** intro Heq_xa_true.
+           rewrite Heq_xa_true in Heq_xa. simpl in Heq_xa.
+           apply beq_nat_false in Heq_xa. auto.
+        ** apply IHxs.
+           unfold mem in Hxs. rewrite Heq_xa in Hxs.
+           auto.
 Qed.
 
-Lemma in_implies_mem_true :
+Lemma in_iff_mem_true :
   forall x xs,
-    In x xs -> mem x xs = true.
+    In x xs <-> mem x xs = true.
 Proof.
-  intros.
-  induction xs.
-  - exfalso. apply (in_nil H).
-  - simpl.
-    destruct (x =? a) eqn:Heq_xa.
-    + reflexivity.
-    + apply IHxs. apply in_inv in H. destruct H.
-      * exfalso. rewrite beq_nat_false_iff in Heq_xa.
-        apply Heq_xa. symmetry. apply H.
-      * apply H.
+  intros. split.
+  - intro Hxs.
+    induction xs.
+    + auto.
+    + simpl.
+      destruct (x =? a) eqn:Heq_xa.
+      * reflexivity.
+      * apply IHxs. apply in_inv in Hxs. destruct Hxs.
+        ** exfalso. rewrite beq_nat_false_iff in Heq_xa.
+           apply Heq_xa. symmetry. auto.
+        ** auto.
+  - intro Hxs.
+    induction xs.
+    + discriminate Hxs.
+    + simpl.
+      destruct (x =? a) eqn:Heq_xa.
+      * left. symmetry. apply beq_nat_true in Heq_xa. auto.
+      * right. apply IHxs.
+        unfold mem in Hxs.
+        rewrite Heq_xa in Hxs. auto.
 Qed.
 
 End Util.
